fairis/heap_lang/examples/mu_role.v
@@ -29,4 +29,26 @@ Section MuRole.
     by iApply "MU".
   Qed.
 
+  (* Definition MU__drop ρ E P: iProp Σ :=   *)
+  (*   ∀ τ f R, τ ↦M ({[ ρ := f ]} ∪ (S <$> R)) ∗ ⌜ ρ ∉ dom R ⌝ -∗ *)
+  (*             MU E τ (τ ↦M R ∗ P) (LM := LM). *)
+
+  (* Lemma MU__r_wand E ρ (P Q: iProp Σ): *)
+  (*   (P -∗ Q) -∗ MU__r ρ E P -∗ MU__r ρ E Q. *)
+  (* Proof. *)
+  (*   iIntros "HPQ HMU". rewrite /MU__r. iIntros "**". *)
+  (*   iSpecialize ("HMU" with "[$]").  *)
+  (*   iApply (MU_wand with "[HPQ] [$]"). iFrame. *)
+  (*   iIntros "[??]". iFrame. by iApply "HPQ".  *)
+  (* Qed. *)
+
+  (* Lemma MU__r_mask_weaken E1 E2 ρ (P: iProp Σ) *)
+  (*   (SUB: E1 ⊆ E2): *)
+  (*   MU__r ρ E1 P -∗ MU__r ρ E2 P. *)
+  (* Proof. *)
+  (*   iIntros "MU". rewrite /MU__r. iIntros "**". *)
+  (*   iApply MU_mask_weaken; eauto. *)
+  (*   by iApply "MU". *)
+  (* Qed. *)
+
 End MuRole.
